Working on a linearlizability proof for the prototype

src/Prototype/Correctness.v
@@ -1,4 +1,4 @@
-Require Import List String Peano_dec.
+Require Import List String Peano_dec Eqdep.
 Require Import FnMap Language SingleValue.
 
 Ltac inv H := inversion H; subst; clear H.
@@ -7,29 +7,92 @@ Ltac dest_in :=
     match goal with
     | [H: In _ _ |- _] => inv H
     end.
+Ltac dest_existT :=
+  repeat match goal with
+         | [H: existT _ _ _ = existT _ _ _ |- _] =>
+           (apply EqdepTheory.inj_pair2 in H; subst)
+         end.
 
-Lemma parent_sequential:
-  forall hst,
-    HistoryOf (existT (fun st => Object SingleValueMsg st) ParentState parent :: nil) hst ->
-    Sequential hst.
-Proof.
-  unfold HistoryOf; intros.
-  destruct H as [oss [oims ?]].
-Admitted.
+Section ParentSequential.
+
+  Definition parentObj :=
+    existT (fun st => Object SingleValueMsg st) ParentState parent :: nil.
+
+  Lemma parent_sequential':
+    forall hst oss1 msgs1 oss2 msgs2,
+      steps parentObj oss1 msgs1 hst oss2 msgs2 ->
+      forall pos ss,
+        find parentIdx oss1 = Some (existT _ (ParentState: Type) pos) ->
+        ss = match ps_request_from (os_state pos) with
+             | Some (from, _) => Some (from, parentIdx)
+             | None => None
+             end ->
+        Sequential' (intHistory (getIndices parentObj) hst) ss.
+  Proof.
+    induction 1; simpl; intros; auto; subst.
+
+    inv H0; inv H6.
+    - (* internal *)
+      inv H2; [|inv H6].
+      pose proof (eq_sigT_fst H6); subst; dest_existT.
+
+      specialize (IHsteps _ _ H1 eq_refl).
+
+      simpl in H3.
+      remember (ParentGetReq msg_in (os_state os)) as getReqV; destruct getReqV.
+      + (* getReq *)
+        inv H3.
+        destruct msg_in as [msg_in_type msg_in_from msg_in_to msg_in_content]; simpl in *.
+        unfold ParentGetReq in HeqgetReqV; simpl in HeqgetReqV.
+        remember (from_external msg_in_from) as msg_in_from_ext.
+        destruct msg_in_from_ext; try discriminate.
+        destruct msg_in_content; try discriminate.
+        remember (os_state os) as oss.
+        destruct oss as [oss_is_valid oss_value oss_request_from]; simpl in *.
+        destruct oss_request_from; try discriminate.
+        destruct oss_is_valid; inv HeqgetReqV; simpl in *.
+        * admit.
+        * admit.
+        
+      + remember (ParentSetReq msg_in (os_state os)) as setReqV; destruct setReqV.
+        * (* setReq *)
+          admit.
+        * remember (ParentInvResp msg_in (os_state os)) as invRespV;
+            destruct invRespV; [|discriminate].
+          (* invResp *)
+          admit.
+
+    - (* external: contradiction *)
+      exfalso; admit.
+    
+  Admitted.
   
-Lemma parent_linear:
-  Linear (existT (fun st => Object SingleValueMsg st) ParentState parent :: nil).
+  Lemma parent_intHistory_sequential:
+    forall hst,
+      HistoryOf parentObj hst ->
+      Sequential (intHistory (getIndices parentObj) hst).
+  Proof.
+    unfold HistoryOf, Sequential; intros.
+    destruct H as [oss [oims ?]].
+    eapply parent_sequential' in H; eauto; reflexivity.
+  Qed.
+
+End ParentSequential.
+  
+Lemma parent_intLinear:
+  IntLinear (existT (fun st => Object SingleValueMsg st) ParentState parent :: nil).
 Proof.
-  unfold Linear; intros.
+  unfold IntLinear, AbsLinear; intros.
   exists (complete hst); split; auto.
   - admit. (* HistoryOf hst -> HistoryOf (complete hst) *)
-  - unfold Linearlizable'; split; auto.
+  - rewrite intHistory_complete_comm.
+    unfold Linearlizable'; split; auto.
     apply sequential_complete.
-    apply parent_sequential; auto.
+    apply parent_intHistory_sequential; auto.
 Admitted.
 
-Lemma child_linear: forall i,
-    Linear (existT (fun st => Object SingleValueMsg st) ChildState (child i) :: nil).
+Lemma child_intLinear:
+  forall i, IntLinear (existT (fun st => Object SingleValueMsg st) ChildState (child i) :: nil).
 Proof.
 Admitted.
 
@@ -37,8 +100,8 @@ Theorem impl_linear: ExtLinear impl.
 Proof.
   apply extLinear_local.
   intros; dest_in.
-  - apply parent_linear.
-  - apply child_linear.
-  - apply child_linear.
+  - apply parent_intLinear.
+  - apply child_intLinear.
+  - apply child_intLinear.
 Qed.  
 
